@prefix owl: <http://www.w3.org/2002/07/owl#> .
@prefix xsd: <http://www.w3.org/2001/XMLSchema#> .
@prefix skos: <http://www.w3.org/2004/02/skos/core#> .
@prefix schemas: <https://schema.org/> .
@prefix dcterms: <http://purl.org/dc/terms/> .
@prefix rov: <http://www.w3.org/ns/regorg#> .

<https://vocab.belgif.be/auth/IMKL-WaterSubthemeValue> a skos:ConceptScheme;
  dcterms:title "IMKL-WaterSubthemeValue"@en, "IMKL-WaterSubthemeValue"@nl;
  dcterms:description "Classification of water subthemes."@en;
  dcterms:description "Classificatie van water subthema's."@nl;
  dcterms:creator <https://org.belgif.be/id/CbeRegisteredEntity/0795547478>;
  dcterms:rightsHolder <https://org.belgif.be/id/CbeRegisteredEntity/0795547478>;
  owl:versionInfo "3.0";
  dcterms:modified "2025-02-13"^^xsd:date;
  dcterms:source <https://github.com/belgif/ICEGthema-imkl> .

<https://org.belgif.be/id/CbeRegisteredEntity/0795547478> rov:legalName "Vlaams Datanutsbedrijf"@en, "Vlaams Datanutsbedrijf"@nl .

<https://vocab.belgif.be/auth/IMKL-WaterSubthemeValue/drinkingWaterDistribution> a skos:Concept;
  skos:inScheme <https://vocab.belgif.be/auth/IMKL-WaterSubthemeValue>;
  skos:notation "drinkingWaterDistribution";
  skos:prefLabel "Drinking water distribution"@en;
  skos:prefLabel "Drinkwater distributie"@nl;
  dcterms:description """Regardless of its diameter, the main purpose of a distribution pipeline is to provide local distribution of drinking water by distributing the supplied water directly to a large number of individual household and non-household final customers."""@en;
  dcterms:description """Een distributieleiding heeft, onafhankelijk van de diameter, als voornaamste doel de lokale verdeling van het drinkwater te verzorgen door het aangevoerde water rechtstreeks over een groot aantal individuele huishoudelijke- en niet-huishoudelijke eindafnemers te verdelen."""@nl;
  schemas:startDate "2024-01-01"^^xsd:date;
  schemas:endDate "9999-12-31"^^xsd:date .
  
<https://vocab.belgif.be/auth/IMKL-WaterSubthemeValue/drinkingWaterSupply> a skos:Concept;
  skos:inScheme <https://vocab.belgif.be/auth/IMKL-WaterSubthemeValue>;
  skos:notation "drinkingWaterSupply";
  skos:prefLabel "Drinking water supply"@en;
  skos:prefLabel "Drinkwater toevoer"@nl;
  dcterms:description """A supply pipeline, irrespective of its diameter, has one of the following purposes :
The supply of demarcated distribution areas, whether they are of a domestic, industrial or agricultural nature or a mixture thereof;
The security connections between and within distribution areas, with the aim of ensuring the supplied capacities of these distribution areas;
The transport of drinking water between water production centres and between the water extractions and these water distribution centres;
The transport of drinking water to large customers (port areas, a large company, an airport,...)"""@en;
  dcterms:description """Een toevoerleiding heeft, onafhankelijk van de diameter, één van volgende doelen :
•	De bevoorrading van afgelijnde distributiegebieden, ongeacht deze een huishoudelijk, industrieel of landbouwkarakter hebben of een mengvorm ervan;
•	De veiligheidsverbindingen tussen  en in de distributiegebieden, met als doel het verzekeren van de aangevoerde capaciteiten van deze distributiegebieden;
•	Het vervoer van drinkwater  tussen waterproductiecentra onderling en tussen de waterwinningen en deze waterprodcutiecentra;
•	Het vervoer van drinkwater naar grote klanten (havenzones, een groot bedrijf, een luchthaven,..)"""@nl;
  schemas:startDate "2024-01-01"^^xsd:date;
  schemas:endDate "9999-12-31"^^xsd:date .
  
