@prefix owl: <http://www.w3.org/2002/07/owl#> .
@prefix xsd: <http://www.w3.org/2001/XMLSchema#> .
@prefix skos: <http://www.w3.org/2004/02/skos/core#> .
@prefix schemas: <https://schema.org/> .
@prefix dcterms: <http://purl.org/dc/terms/> .

<https://vocab.belgif.be/auth/IMKL-OilGasChemicalsSubthemeValue> a skos:ConceptScheme;
  dcterms:title "IMKL-OilGasChemicalsSubthemeValue"@en;
  dcterms:description "Classification of oil, gas, chemicals subthemes."@en;
  dcterms:creator <https://org.belgif.be/id/CbeRegisteredEntity/0795547478>;
  dcterms:rightsHolder <https://org.belgif.be/id/CbeRegisteredEntity/0795547478>;
  owl:versionInfo "3.0";
  dcterms:modified "2024-09-26"^^xsd:date;
  dcterms:source <https://github.com/belgif/ICEGthema-imkl> .

<https://org.belgif.be/id/CbeRegisteredEntity/0795547478> rov:legalName "Vlaams Datanutsbedrijf"@en .

<https://vocab.belgif.be/auth/IMKL-OilGasChemicalsSubthemeValue/naturalGasDistributionLowPressure> a skos:Concept;
  skos:inScheme <https://vocab.belgif.be/auth/IMKL-OilGasChemicalsSubthemeValue>;
  skos:notation "naturalGasDistributionLowPressure";
  skos:prefLabel "naturalGasDistributionLowPressure"@en;
  dct:description "Pipe whose highest permissible operating pressure does not exceed 0.1 kgf/cm2 (98.07 mbar)."@en;
  schemas:startDate "2024-01-01"^^xsd:date;
  schemas:endDate "9999-12-31"^^xsd:date .
  
<https://vocab.belgif.be/auth/IMKL-OilGasChemicalsSubthemeValue/naturalGasDistributionMediumPressure> a skos:Concept;
  skos:inScheme <https://vocab.belgif.be/auth/IMKL-OilGasChemicalsSubthemeValue>;
  skos:notation "naturalGasDistributionMediumPressure";
  skos:prefLabel "naturalGasDistributionMediumPressure"@en;
  dct:description "Pipe whose highest allowable operating pressure exceeds 0.1 kgf/cm2 (98.07 mbar) without exceeding 15 kgf/cm2 (14.71 bar)."@en;
  schemas:startDate "2024-01-01"^^xsd:date;
  schemas:endDate "9999-12-31"^^xsd:date .
  
<https://vocab.belgif.be/auth/IMKL-OilGasChemicalsSubthemeValue/naturalGasTransport> a skos:Concept;
  skos:inScheme <https://vocab.belgif.be/auth/IMKL-OilGasChemicalsSubthemeValue>;
  skos:notation "naturalGasTransport";
  skos:prefLabel "naturalGasTransport"@en;
  dct:description "Natural gas transmission network - installations subject to law 12/04/65."@en;
  schemas:startDate "2024-01-01"^^xsd:date;
  schemas:endDate "9999-12-31"^^xsd:date .
  
<https://vocab.belgif.be/auth/IMKL-OilGasChemicalsSubthemeValue/oilGasChemicalsTransport> a skos:Concept;
  skos:inScheme <https://vocab.belgif.be/auth/IMKL-OilGasChemicalsSubthemeValue>;
  skos:notation "oilGasChemicalsTransport";
  skos:prefLabel "oilGasChemicalsTransport"@en;
  dct:description "Transmission network for transporting products other than natural gas - installations subject to law 12/04/65."@en;
  schemas:startDate "2024-01-01"^^xsd:date;
  schemas:endDate "9999-12-31"^^xsd:date .
  
